final(?) refactoring

WebAssembly/Wasm_Interpreter.thy
@@ -634,8 +634,8 @@ function(sequential) run_iter :: "fuel \<Rightarrow> config \<Rightarrow> res_tu
 termination
   by (relation "measure (\<lambda>p. fst p)") auto
 
-fun run_v :: "fuel \<Rightarrow> depth \<Rightarrow> s \<Rightarrow> f \<Rightarrow> b_e list \<Rightarrow> (s \<times> res)" where
-  "run_v n d s f b_es =
+fun run_v :: "fuel \<Rightarrow> depth \<Rightarrow> (s \<times> f \<times> b_e list) \<Rightarrow> (s \<times> res)" where
+  "run_v n d (s, f, b_es) =
      (let (cfg',res) = run_iter n (Config d s (Frame_context (Redex [] [] b_es) [] 0 f) []) in
       case cfg' of (Config d s fc fcs) \<Rightarrow> (s,res))"
 
